coq/extracted/rooplRun.mli
@@ -1,0 +1,207 @@
+
+type nat =
+| O
+| S of nat
+
+val length : 'a1 list -> nat
+
+val app : 'a1 list -> 'a1 list -> 'a1 list
+
+type comparison =
+| Eq
+| Lt
+| Gt
+
+val compOpp : comparison -> comparison
+
+val add : nat -> nat -> nat
+
+type positive =
+| XI of positive
+| XO of positive
+| XH
+
+type n =
+| N0
+| Npos of positive
+
+type z =
+| Z0
+| Zpos of positive
+| Zneg of positive
+
+module Nat :
+ sig
+  val eqb : nat -> nat -> bool
+
+  val leb : nat -> nat -> bool
+
+  val ltb : nat -> nat -> bool
+
+  val eq_dec : nat -> nat -> bool
+ end
+
+module Pos :
+ sig
+  val succ : positive -> positive
+
+  val add : positive -> positive -> positive
+
+  val add_carry : positive -> positive -> positive
+
+  val pred_double : positive -> positive
+
+  val pred_N : positive -> n
+
+  val mul : positive -> positive -> positive
+
+  val compare_cont : comparison -> positive -> positive -> comparison
+
+  val compare : positive -> positive -> comparison
+
+  val eqb : positive -> positive -> bool
+
+  val coq_Nsucc_double : n -> n
+
+  val coq_Ndouble : n -> n
+
+  val coq_lxor : positive -> positive -> n
+
+  val iter_op : ('a1 -> 'a1 -> 'a1) -> positive -> 'a1 -> 'a1
+
+  val to_nat : positive -> nat
+ end
+
+module N :
+ sig
+  val succ_pos : n -> positive
+
+  val coq_lxor : n -> n -> n
+ end
+
+module Z :
+ sig
+  val double : z -> z
+
+  val succ_double : z -> z
+
+  val pred_double : z -> z
+
+  val pos_sub : positive -> positive -> z
+
+  val add : z -> z -> z
+
+  val opp : z -> z
+
+  val sub : z -> z -> z
+
+  val mul : z -> z -> z
+
+  val compare : z -> z -> comparison
+
+  val ltb : z -> z -> bool
+
+  val eqb : z -> z -> bool
+
+  val to_nat : z -> nat
+
+  val of_N : n -> z
+
+  val coq_lxor : z -> z -> z
+ end
+
+val map : ('a1 -> 'a2) -> 'a1 list -> 'a2 list
+
+val in_dec : ('a1 -> 'a1 -> bool) -> 'a1 -> 'a1 list -> bool
+
+type id = nat
+
+type mid = nat
+
+type loc = nat
+
+type field = nat
+
+type cid = nat
+
+type state = { vs : (id -> z); os : (id -> loc option); hn : nat;
+               hp : (loc -> field -> z); hc : (loc -> cid) }
+
+val setv : state -> id -> z -> state
+
+type binop =
+| Oadd
+| Osub
+| Omul
+| Oeq
+| Olt
+
+type exp =
+| Cst of z
+| Var of id
+| Fld of id * field
+| Idx of id * exp
+| Bop of binop * exp * exp
+
+val bval : bool -> z
+
+val eval_binop : binop -> z -> z -> z
+
+val rdf : state -> id -> field -> z
+
+val eval : exp -> state -> z
+
+val fv : exp -> id list
+
+type modop =
+| MAdd
+| MSub
+| MXor
+
+val mapp : modop -> z -> z -> z
+
+val minv : modop -> modop
+
+type stm =
+| Sskip
+| Sassign of id * modop * exp
+| Sfassign of id * field * modop * exp
+| Saassign of id * exp * modop * exp
+| Sswap of id * id
+| Saswap of id * exp * id * exp
+| Soswap of id * id
+| Scopy of id * id
+| Suncopy of id * id
+| Sseq of stm * stm
+| Sif of exp * stm * stm * exp
+| Sloop of exp * stm * stm * exp
+| Slocal of id * exp * stm * exp
+| Sshow of exp
+| Sobj of cid * id * stm
+| Scall of mid * id list
+| Suncall of mid * id list
+| Socall of id * mid * id list
+| Souncall of id * mid * id list
+
+val invert : stm -> stm
+
+val mk_ren : id list -> id list -> id -> id
+
+val rename_exp : (id -> id) -> exp -> exp
+
+val rename : (id -> id) -> stm -> stm
+
+type mdecl =
+| MDecl of id list * stm
+
+type cdecl =
+| CDecl of cid option * (mid -> mdecl option)
+
+type ctable = cid -> cdecl option
+
+type menv = { procs : (mid -> mdecl option); classes : ctable }
+
+val run : nat -> menv -> stm -> state -> state option
+
+val run_loop :
+  nat -> menv -> exp -> stm -> stm -> exp -> state -> state option
